Update ReorderCancel

src/prop/Pred.v
@@ -243,6 +243,12 @@ Section Pred.
     | _ => False
     end.
 
+  Definition is_reserve (te: ThreadEvent.t): Prop :=
+    match te with
+    | ThreadEvent.promise _ _ _ Message.reserve Memory.op_kind_add => True
+    | _ => False
+    end.
+
 End Pred.
 
 Section PredStep.
