src/prop/ReorderCancel.v
@@ -40,9 +40,6 @@ Lemma reorder_read_cancel
       loc2 to2 val2 released2 ord2
       (STEP1: Local.read_step lc0 mem0 loc2 to2 val2 released2 ord2 lc1)
       (STEP2: Local.promise_step lc1 mem0 loc1 from1 to1 msg1 lc2 mem1 Memory.op_kind_cancel)
-  (* (LOCAL0: Local.wf lc0 mem0) *)
-  (* (MEM0: Memory.closed mem0) *)
-  (* (LOCTS: (loc1, to1) <> (loc2, to2)): *)
   :
     exists lc1',
       (<<STEP1: Local.promise_step lc0 mem0 loc1 from1 to1 msg1 lc1' mem1 Memory.op_kind_cancel>>) /\
@@ -104,9 +101,9 @@ Lemma reorder_write_cancel
       (STEP1: Local.write_step lc0 sc0 mem0 loc2 from2 to2 val2 releasedm2 released2 ord2 lc1 sc2 mem1 kind2)
       (STEP2: Local.promise_step lc1 mem1 loc1 from1 to1 msg1 lc2 mem2 Memory.op_kind_cancel)
   :
-    exists kind2' lc1' mem1',
-      (exists from1', <<STEP2: Local.promise_step lc0 mem0 loc1 from1' to1 msg1 lc1' mem1' Memory.op_kind_cancel>>) /\
-      (<<STEP2: Local.write_step lc1' sc0 mem1' loc2 from2 to2 val2 releasedm2 released2 ord2 lc2 sc2 mem2 kind2'>>).
+    exists lc1' mem1',
+      (<<STEP1: Local.promise_step lc0 mem0 loc1 from1 to1 msg1 lc1' mem1' Memory.op_kind_cancel>>) /\
+      (<<STEP2: Local.write_step lc1' sc0 mem1' loc2 from2 to2 val2 releasedm2 released2 ord2 lc2 sc2 mem2 kind2>>).
 Proof.
   inv STEP2. inv PROMISE.
   inv STEP1. ss. inv WRITE.
@@ -202,355 +199,125 @@ Proof.
       erewrite Memory.bot_get in *. ss.
 Qed.
 
-Lemma reorder_pf_step_cancel
+Lemma reorder_step_cancel
       lang
-      e1 e2 th0 th1 th2
-      (STEP1: @pred_step (promise_free /1\ (fun e => ~ is_cancel e)) lang
-                         e1 th0 th1)
-      (STEP2: pred_step is_cancel e2 th1 th2)
+      pf1 pf2 e1 e2 th0 th1 th2
+      (STEP1: @Thread.step lang pf1 e1 th0 th1)
+      (STEP2: Thread.step pf2 e2 th1 th2)
+      (CANCEL: is_cancel e2)
       (LOCAL: Local.wf th0.(Thread.local) th0.(Thread.memory))
       (MEMORY: Memory.closed th0.(Thread.memory)):
-  exists e2' e1' th1',
-    (<<STEP1: pred_step is_cancel e2' th0 th1'>>) /\
-    (<<STEP2: pred_step (promise_free /1\ (fun e => ~ is_cancel e)) e1' th1' th2>>) /\
-    (<<EVT: ThreadEvent.get_machine_event e1' = ThreadEvent.get_machine_event e1>>)
+  (exists th1',
+    (<<STEP1: Thread.step pf2 e2 th0 th1'>>) /\
+    (<<STEP2: Thread.step pf1 e1 th1' th2>>)) \/
+  (th2 = th0 /\ <<RESERVE: is_reserve e1>>)
 .
 Proof.
-  inv STEP1. inv STEP2. des. unfold is_cancel in SAT0. des_ifs.
-  inv STEP0. inv STEP1; inv STEP0; [|inv LOCAL0]. ss.
-  inv STEP. inv STEP0; ss.
+  unfold is_cancel in *. des_ifs.
+  inv STEP2; inv STEP; [|inv LOCAL0]. ss.
+  inv STEP1; ss.
   - inv STEP. ss. exploit reorder_promise_promise_cancel; eauto.
-    { des_ifs. inv LOCAL1. inv PROMISE; ss. }
-    i. des; clarify. esplits.
-    + econs.
-      * econs. econs 1. econs; eauto.
-      * ss.
-    + econs.
-      * econs. econs 1. econs; eauto.
-      * ss.
-    + ss.
-  - inv STEP. ss. inv LOCAL1; ss.
+    i. des; clarify; eauto.
+    left. esplits.
+    + econs 1. econs; eauto.
+    + econs 1. econs; eauto.
+  - left. inv STEP. ss. inv LOCAL1; ss.
     + esplits.
-      * econs.
-        { econs. econs 1. econs; eauto. }
-        { ss. }
-      * econs.
-        { econs. econs 2. econs; eauto; ss. }
-        { ss. }
-      * ss.
+      * econs 1. econs; eauto.
+      * econs 2. econs; eauto; ss.
     + exploit reorder_read_cancel; eauto. i. des. esplits.
-      * econs.
-        { econs. econs 1. econs; eauto. }
-        { ss. }
-      * econs.
-        { econs. econs 2. econs; eauto; ss. }
-        { ss. }
-      * ss.
+      * econs 1. econs; eauto.
+      * econs 2. econs; eauto; ss.
     + exploit reorder_write_cancel; eauto. i. des. esplits.
-      * econs.
-        { econs. econs 1. econs; eauto. }
-        { ss. }
-      * econs.
-        { econs. econs 2. econs; eauto; ss. }
-        { ss. }
-      * ss.
+      * econs 1. econs; eauto.
+      * econs 2. econs; eauto; ss.
     + exploit reorder_write_cancel; eauto. i. des.
       exploit reorder_read_cancel; eauto. i. des.
       esplits.
-      * econs.
-        { econs. econs 1. econs; eauto. }
-        { ss. }
-      * econs.
-        { econs. econs 2. econs; eauto; ss. }
-        { ss. }
-      * ss.
+      * econs 1. econs; eauto.
+      * econs 2. econs; eauto; ss.
     + exploit reorder_fence_cancel; eauto. i. des. esplits.
-      * econs.
-        { econs. econs 1. econs; eauto. }
-        { ss. }
-      * econs.
-        { econs. econs 2. econs; eauto; ss. }
-        { ss. }
-      * ss.
+      * econs 1. econs; eauto.
+      * econs 2. econs; eauto; ss.
     + exploit reorder_fence_cancel; eauto. i. des. esplits.
-      * econs.
-        { econs. econs 1. econs; eauto. }
-        { ss. }
-      * econs.
-        { econs. econs 2. econs; eauto; ss. eauto. }
-        { ss. }
-      * ss.
+      * econs 1. econs; eauto.
+      * econs 2. econs; eauto; ss.
     + esplits.
-      * econs; eauto.
-        { econs. econs 1. econs; eauto. }
-        { ss. }
-      * econs.
-        { econs. econs 2. econs.
-          - instantiate (1:=ThreadEvent.failure). auto.
-          - econs. econs. inv LOCAL2. inv LOCAL0. inv PROMISE.
-            ii. ss. erewrite Memory.remove_o in PROMISE; eauto. des_ifs.
-            eapply CONSISTENT; eauto. }
-        { ss. }
-      * ss.
+      * econs 1. econs; eauto.
+      * econs 2. econs; eauto.
+        econs. econs. inv LOCAL2. inv LOCAL0. inv PROMISE.
+        ii. ss. erewrite Memory.remove_o in PROMISE; eauto. des_ifs.
+        eapply CONSISTENT; eauto.
 Qed.
 
-Lemma reorder_pf_step_cancels
+Lemma reorder_step_cancels
       lang
-      e1 th0 th1 th2
-      (STEP1: @pred_step (promise_free /1\ (fun e => ~ is_cancel e)) lang
-                         e1 th0 th1)
-      (STEPS2: rtc (tau (@pred_step is_cancel _)) th1 th2)
+      pf e1 th0 th1 th2
+      (STEP1: Thread.step pf e1 th0 th1)
+      (STEPS2: rtc (@Thread.cancel_step lang) th1 th2)
       (LOCAL: Local.wf th0.(Thread.local) th0.(Thread.memory))
       (MEMORY: Memory.closed th0.(Thread.memory))
       (SC: Memory.closed_timemap (Thread.sc th0) (Thread.memory th0))
   :
-    exists e1' th1',
-      (<<STEPS1: rtc (tau (@pred_step is_cancel _)) th0 th1'>>) /\
-      (<<STEP2: pred_step (promise_free /1\ (fun e => ~ is_cancel e)) e1' th1' th2>>) /\
-      (<<EVT: ThreadEvent.get_machine_event e1' = ThreadEvent.get_machine_event e1>>)
+    (exists th1',
+        (<<STEPS1: rtc (@Thread.cancel_step lang) th0 th1'>>) /\
+        (<<STEP2: Thread.step pf e1 th1' th2>>)) \/
+    ((<<STEPS1: rtc (@Thread.cancel_step lang) th0 th2>>) /\ (<<RESERVE: is_reserve e1>>))
 .
 Proof.
   ginduction STEPS2; i.
   - esplits; eauto.
-  - inv H. exploit reorder_pf_step_cancel.
+  - inv H. exploit reorder_step_cancel.
     { eapply STEP1. }
-    { eapply TSTEP. }
+    { eapply STEP. }
+    { ss. }
     { eauto. }
     { eauto. }
     i. des.
-    dup STEP0. inv STEP3. inv STEP. exploit Thread.step_future.
-    { eapply STEP3. }
-    { eauto. }
-    { eauto. }
-    { eauto. } i. des.
-    exploit IHSTEPS2; eauto. i. des.
-    esplits.
-    + econs 2.
-      * econs; eauto.
-        unfold is_cancel in SAT. des_ifs.
-      * eauto.
-    + eauto.
-    + etrans; eauto.
-Qed.
-
-Lemma pf_steps_cancels_not_cancels
-      lang th0 th2
-      (STEPS: rtc (tau (@pred_step promise_free lang)) th0 th2)
-      (LOCAL: Local.wf th0.(Thread.local) th0.(Thread.memory))
-      (MEMORY: Memory.closed th0.(Thread.memory))
-      (SC: Memory.closed_timemap (Thread.sc th0) (Thread.memory th0))
-  :
-    exists th1,
-      (<<STEPS1: rtc (tau (@pred_step is_cancel _)) th0 th1>>) /\
-      (<<STEPS2: rtc (tau (@pred_step (promise_free /1\ (fun e => ~ is_cancel e)) _)) th1 th2>>)
-.
-Proof.
-  ginduction STEPS; i.
-  - esplits; eauto.
-  - inv H. dup TSTEP. inv TSTEP0. inv STEP.
-    exploit Thread.step_future; eauto. i. des.
-    exploit IHSTEPS; eauto. i. des.
-    destruct (classic (is_cancel e)).
-    + esplits.
-      * econs 2.
-        { econs.
-          - econs; eauto.
-            econs. eapply STEP0.
-          - unfold is_cancel in H. des_ifs. }
-        { eapply STEPS1. }
-      * eapply STEPS2.
-    + exploit reorder_pf_step_cancels.
-      { econs.
-        - econs. eapply STEP0.
-        - splits; auto. }
-      { eapply STEPS1. }
-      { eauto. }
-      { eauto. }
-      { eauto. }
-      i. des. esplits.
-      * eauto.
-      * econs 2.
-        { econs; eauto. etrans; eauto. }
-        { eauto. }
-Qed.
-
-
-Lemma reorder_pf_step_cancel_no_sc
-      lang
-      e1 e2 th0 th1 th2
-      (STEP1: @pred_step (no_sc /1\ (fun e => ~ is_cancel e)) lang
-                         e1 th0 th1)
-      (STEP2: pred_step is_cancel e2 th1 th2)
-      (LOCAL: Local.wf th0.(Thread.local) th0.(Thread.memory))
-      (MEMORY: Memory.closed th0.(Thread.memory)):
-  exists e2' e1' th1',
-    (<<STEP1: opt_pred_step is_cancel e2' th0 th1'>>) /\
-    (<<STEP2: opt_pred_step (no_sc /1\ (fun e => ~ is_cancel e)) e1' th1' th2>>) /\
-    (<<EVT: ThreadEvent.get_machine_event e1' = ThreadEvent.get_machine_event e1>>)
-.
-Proof.
-  inv STEP1. inv STEP2. des. unfold is_cancel in SAT0. des_ifs.
-  inv STEP0. inv STEP1; inv STEP0; [|inv LOCAL0]. ss.
-  inv STEP. inv STEP0; ss.
-  - inv STEP. ss. exploit reorder_promise_promise_cancel; eauto.
-    { des_ifs. inv LOCAL1. inv PROMISE; ss. }
-    i. des; clarify.
-    { esplits.
-      + econs 1.
-      + econs 1.
-      + ss.
-    }
-    { esplits.
-      + econs 2. econs.
-        * econs. econs 1. econs; eauto.
-        * ss.
-      + econs 2. econs.
-        * econs. econs 1. econs; eauto.
-        * ss.
-      + ss.
-    }
-  - inv STEP. ss. inv LOCAL1; ss.
-    + esplits.
-      * econs 2. econs.
-        { econs. econs 1. econs; eauto. }
-        { ss. }
-      * econs 2. econs.
-        { econs. econs 2. econs; eauto; ss. }
-        { ss. }
-      * ss.
-    + exploit reorder_read_cancel; eauto. i. des. esplits.
-      * econs 2. econs.
-        { econs. econs 1. econs; eauto. }
-        { ss. }
-      * econs 2. econs.
-        { econs. econs 2. econs; eauto; ss. }
-        { ss. }
-      * ss.
-    + exploit reorder_write_cancel; eauto. i. des. esplits.
-      * econs 2. econs.
-        { econs. econs 1. econs; eauto. }
-        { ss. }
-      * econs 2. econs.
-        { econs. econs 2. econs; eauto; ss. }
-        { ss. }
-      * ss.
-    + exploit reorder_write_cancel; eauto. i. des.
-      exploit reorder_read_cancel; eauto. i. des.
-      esplits.
-      * econs 2. econs.
-        { econs. econs 1. econs; eauto. }
-        { ss. }
-      * econs 2. econs.
-        { econs. econs 2. econs; eauto; ss. }
-        { ss. }
-      * ss.
-    + exploit reorder_fence_cancel; eauto. i. des. esplits.
-      * econs 2. econs.
-        { econs. econs 1. econs; eauto. }
-        { ss. }
-      * econs 2. econs.
-        { econs. econs 2. econs; eauto; ss. }
-        { ss. }
-      * ss.
-    + esplits.
-      * econs 2. econs; eauto.
-        { econs. econs 1. econs; eauto. }
-        { ss. }
-      * econs 2. econs.
-        { econs. econs 2. econs.
-          - instantiate (1:=ThreadEvent.failure). auto.
-          - econs. econs. inv LOCAL2. inv LOCAL0. inv PROMISE.
-            ii. ss. erewrite Memory.remove_o in PROMISE; eauto. des_ifs.
-            eapply CONSISTENT; eauto. }
-        { ss. }
-      * ss.
-Qed.
-
-Lemma reorder_pf_step_cancels_no_sc
-      lang
-      e1 th0 th1 th2
-      (STEP1: @opt_pred_step (no_sc /1\ (fun e => ~ is_cancel e)) lang
-                         e1 th0 th1)
-      (STEPS2: rtc (tau (@pred_step is_cancel _)) th1 th2)
-      (LOCAL: Local.wf th0.(Thread.local) th0.(Thread.memory))
-      (MEMORY: Memory.closed th0.(Thread.memory))
-      (SC: Memory.closed_timemap (Thread.sc th0) (Thread.memory th0))
-  :
-    exists e1' th1',
-      (<<STEPS1: rtc (tau (@pred_step is_cancel _)) th0 th1'>>) /\
-      (<<STEP2: opt_pred_step (no_sc /1\ (fun e => ~ is_cancel e)) e1' th1' th2>>) /\
-      (<<EVT: ThreadEvent.get_machine_event e1' = ThreadEvent.get_machine_event e1>>)
-.
-Proof.
-  ginduction STEPS2; i.
-  - esplits; eauto.
-  - inv STEP1.
-    { eexists _, z. esplits; eauto. econs. }
-    inv H. exploit reorder_pf_step_cancel_no_sc.
-    { eapply STEP. }
-    { eapply TSTEP. }
-    { eauto. }
-    { eauto. }
-    i. des. inv STEP1.
-    { exploit IHSTEPS2; eauto. i. des.
-      esplits.
-      + eauto.
-      + eauto.
-      + etrans; eauto.
-    }
-    { dup STEP0. inv STEP1. inv STEP3. exploit Thread.step_future.
-      { eapply STEP1. }
-      { eauto. }
-      { eauto. }
-      { eauto. } i. des.
+    { exploit Thread.step_future; try apply STEP0; eauto. i. des.
       exploit IHSTEPS2; eauto. i. des.
-      esplits.
-      + econs 2.
-        * econs; eauto.
-          unfold is_cancel in SAT. des_ifs.
-        * eauto.
-      + eauto.
-      + etrans; eauto.
+      - left. esplits.
+        + econs 2.
+          * splits; auto. econs; eauto.
+          * eauto.
+        + eauto.
+      - right. splits; auto. econs 2; eauto. econs; eauto.
     }
+    { subst. right. esplits; eauto. }
 Qed.
 
-Lemma pf_steps_cancels_not_cancels_no_sc
-      lang th0 th2
-      (STEPS: rtc (tau (@pred_step no_sc lang)) th0 th2)
+Lemma steps_cancels_not_cancels
+      P lang th0 th2
+      (STEPS: rtc (tau (@pred_step P lang)) th0 th2)
       (LOCAL: Local.wf th0.(Thread.local) th0.(Thread.memory))
       (MEMORY: Memory.closed th0.(Thread.memory))
       (SC: Memory.closed_timemap (Thread.sc th0) (Thread.memory th0))
   :
     exists th1,
-      (<<STEPS1: rtc (tau (@pred_step is_cancel _)) th0 th1>>) /\
-      (<<STEPS2: rtc (tau (@pred_step (no_sc /1\ (fun e => ~ is_cancel e)) _)) th1 th2>>)
+      (<<STEPS1: rtc (@Thread.cancel_step _) th0 th1>>) /\
+      (<<STEPS2: rtc (tau (@pred_step (P /1\ fun e => ~ is_cancel e) _)) th1 th2>>)
 .
 Proof.
   ginduction STEPS; i.
   - esplits; eauto.
-  - inv H. dup TSTEP. inv TSTEP0. inv STEP.
+  - inv H. inv TSTEP. inv STEP.
     exploit Thread.step_future; eauto. i. des.
     exploit IHSTEPS; eauto. i. des.
     destruct (classic (is_cancel e)).
-    + esplits.
+    + unfold is_cancel in H. des_ifs. esplits.
       * econs 2.
-        { econs.
-          - econs; eauto.
-            econs. eapply STEP0.
-          - unfold is_cancel in H. des_ifs. }
+        { econs; eauto. }
         { eapply STEPS1. }
       * eapply STEPS2.
-    + exploit reorder_pf_step_cancels_no_sc.
-      { econs 2. econs.
-        - econs. eapply STEP0.
-        - splits; auto. }
+    + exploit reorder_step_cancels.
+      { eapply STEP0. }
       { eapply STEPS1. }
       { eauto. }
       { eauto. }
       { eauto. }
-      i. des. esplits.
+      i. des; eauto. esplits.
       * eauto.
-      * inv STEP2; eauto. econs 2.
-        { econs; eauto. etrans; eauto. }
+      * econs 2.
+        { econs; eauto. econs; eauto. econs; eauto. }
         { eauto. }
 Qed.
